Dafny/examples/BasicBug/simpleBugCompleteLemmas.i.dfy
@@ -1,0 +1,444 @@
+include "simpleBugCode.i.dfy"
+include "simpleBugGeneral.i.dfy"
+include "../../LLVM/llvmREFACTOR.i.dfy"
+include "../../LLVM/types.dfy"
+include "../../Libraries/Seqs.s.dfy"
+
+module simpleBugCompleteLemmas{
+    import opened simpleBugCode
+    import opened simpleBugGeneral
+    import opened LLVM_defRE
+    import opened types
+    import opened Collections__Seqs_s
+
+lemma possibleVulnOutputs(s:state, b:behavior) 
+        requires ValidState(s);
+        requires |b| > 0;
+        requires b[0] == s;
+        requires s.o.Nil?;
+
+        ensures  forall input :: (validInput(s,input) && OperandContents(s,input).val < 2 && BehaviorEvalsCode(codeVuln(input),b)) 
+                                  ==> (behaviorOutput(b) == [Nil,Nil,Nil,Out((Int(1,IntType(1,false)))),Out((Int(1,IntType(1,false))))]);
+        ensures  forall input :: (validInput(s,input) && OperandContents(s,input).val >= 2 && BehaviorEvalsCode(codeVuln(input),b)) 
+                                  ==> (behaviorOutput(b) == [Nil,Nil,Nil,Out((Int(0,IntType(1,false)))),Out((Int(0,IntType(1,false))))]);
+    {
+        var inputWitness := D(Int(1,IntType(4,false)));
+        assert validInput(s,inputWitness);
+        forall input | validInput(s,input) && OperandContents(s,input).val < 2 && BehaviorEvalsCode(codeVuln(input),b)
+            ensures (behaviorOutput(b) == [Nil,Nil,Nil,Out((Int(1,IntType(1,false)))),Out((Int(1,IntType(1,false))))]);
+        {
+            var input :| validInput(s,input) && OperandContents(s,input).val < 2 && BehaviorEvalsCode(codeVuln(input),b);
+            var b' := unwrapVulnBehaviors(s,input);
+            behaviorThatEvalsSameCodeWithSameInitIsEqual(s,codeVuln(input),b');
+        }
+        forall input | validInput(s,input) && OperandContents(s,input).val >= 2 && BehaviorEvalsCode(codeVuln(input),b)
+            ensures (behaviorOutput(b) == [Nil,Nil,Nil,Out((Int(0,IntType(1,false)))),Out((Int(0,IntType(1,false))))]);
+        {
+            var input :| validInput(s,input) && OperandContents(s,input).val >= 2 && BehaviorEvalsCode(codeVuln(input),b);
+            var b' := unwrapVulnBehaviors(s,input);
+            behaviorThatEvalsSameCodeWithSameInitIsEqual(s,codeVuln(input),b');
+        }
+     
+    }
+
+    lemma possibleVulnOutputsWithMiniSpec(s:state, b:behavior)
+        requires ValidState(s);
+        requires |b| > 0;
+        requires b[0] == s;
+        requires s.o.Nil?;
+        ensures  forall input :: (validInput(s,input) && OperandContents(s,input).val < 2 && BehaviorEvalsCode(codeVuln(input),b)) 
+                                  ==> !MiniSpec(b);
+        ensures  forall input :: (validInput(s,input) && OperandContents(s,input).val >= 2 && BehaviorEvalsCode(codeVuln(input),b)) 
+                                  ==> MiniSpec(b);
+        ensures forall input :: ( validInput(s,input) && BehaviorEvalsCode(codeVuln(input),b)) ==> 
+                        (!MiniSpec(b) <==> (behaviorOutput(b) == [Nil,Nil,Nil,Out((Int(1,IntType(1,false)))),Out((Int(1,IntType(1,false))))]));
+         ensures forall input :: ( validInput(s,input) && BehaviorEvalsCode(codeVuln(input),b)) ==> 
+                        (MiniSpec(b) <==> (behaviorOutput(b) == [Nil,Nil,Nil,Out((Int(0,IntType(1,false)))),Out((Int(0,IntType(1,false))))]));
+    {
+        // possibleVulnOutputs(s,b);
+        var inputWitness := D(Int(1,IntType(4,false)));
+        assert validInput(s,inputWitness);
+        forall input | validInput(s,input) && OperandContents(s,input).val < 2 && BehaviorEvalsCode(codeVuln(input),b)
+            ensures !MiniSpec(b);
+            ensures (behaviorOutput(b) == [Nil,Nil,Nil,Out((Int(1,IntType(1,false)))),Out((Int(1,IntType(1,false))))]);
+            ensures !MiniSpec(b) ==> (behaviorOutput(b) == [Nil,Nil,Nil,Out((Int(1,IntType(1,false)))),Out((Int(1,IntType(1,false))))]);
+        {
+            var input :| validInput(s,input) && OperandContents(s,input).val < 2 && BehaviorEvalsCode(codeVuln(input),b);
+            var b' := unwrapVulnBehaviors(s,input);
+            behaviorThatEvalsSameCodeWithSameInitIsEqual(s,codeVuln(input),b');
+            assert !MiniSpec(b);
+            assert (behaviorOutput(b) == [Nil,Nil,Nil,Out((Int(1,IntType(1,false)))),Out((Int(1,IntType(1,false))))]);
+        }
+        forall input | validInput(s,input) && OperandContents(s,input).val >= 2 && BehaviorEvalsCode(codeVuln(input),b)
+            ensures MiniSpec(b);
+            ensures !(behaviorOutput(b) == [Nil,Nil,Nil,Out((Int(1,IntType(1,false)))),Out((Int(1,IntType(1,false))))]);
+            ensures MiniSpec(b) <==> (behaviorOutput(b) == [Nil,Nil,Nil,Out((Int(0,IntType(1,false)))),Out((Int(0,IntType(1,false))))]);
+        {
+            var input :| validInput(s,input) && OperandContents(s,input).val >= 2 && BehaviorEvalsCode(codeVuln(input),b);
+            var b' := unwrapVulnBehaviors(s,input);
+            behaviorThatEvalsSameCodeWithSameInitIsEqual(s,codeVuln(input),b');
+            assert MiniSpec(b);
+            assert (behaviorOutput(b) == [Nil,Nil,Nil,Out((Int(0,IntType(1,false)))),Out((Int(0,IntType(1,false))))]);
+            assert !(behaviorOutput(b) == [Nil,Nil,Nil,Out((Int(1,IntType(1,false)))),Out((Int(1,IntType(1,false))))]);
+        }
+        // assert !MiniSpec(b) ==> (behaviorOutput(b) == [Nil,Nil,Nil,Out((Int(1,IntType(1,false)))),Out((Int(1,IntType(1,false))))]);
+    }
+    lemma constrainedBehaviorSet(s:state,vulnBehaviors:seq<behavior>,patchBehaviors:seq<behavior>,vulnOut:seq<seq<output>>)
+        requires nonTrivialBehaviorPreconditions(s,vulnBehaviors,patchBehaviors)
+        requires vulnOut == allBehaviorOutput(vulnBehaviors);
+        ensures forall p :: (behaviorOutput(p) in vulnOut && !MiniSpec(p)) ==> behaviorOutput(p) in vulnOut;
+        {
+            reveal_nonTrivialBehaviorPreconditionsVuln();
+            reveal_nonTrivialBehaviorPreconditionsPatch();
+            reveal_behaviorOutput();
+            forall p | behaviorOutput(p) in vulnOut
+                ensures !MiniSpec(p) ==> behaviorOutput(p) in vulnOut;
+            {
+                if (MiniSpec(p)){
+                    assert behaviorOutput(p) in vulnOut;
+                }else{
+                    assert !MiniSpec(p);
+                    assert behaviorOutput(p) in vulnOut;
+                }
+            }
+        }
+
+    lemma allOutputConstrainedImpliesSameBehaviorOExists(s:state,vulnBehaviors:seq<behavior>,patchBehaviors:seq<behavior>,vulnOut:seq<seq<output>>)
+        requires nonTrivialBehaviorPreconditions(s,vulnBehaviors,patchBehaviors)
+        requires vulnOut == allBehaviorOutput(vulnBehaviors);
+        ensures forall v :: v in vulnBehaviors ==> (!MiniSpec(v) ==> (behaviorOutput(v) == [Nil,Nil,Nil,Out((Int(1,IntType(1,false)))),Out((Int(1,IntType(1,false))))]));
+        ensures forall p :: constrainedBehavorSet(p,vulnOut) ==> existsSameOutput(vulnBehaviors,p);
+    {
+        reveal_nonTrivialBehaviorPreconditionsVuln();
+        reveal_nonTrivialBehaviorPreconditionsPatch();
+        // reveal_existsSameOutput();
+        // reveal_behaviorOutput();
+        assert forall v :: v in vulnBehaviors  ==> (exists input :: ( validInput(s,input) && BehaviorEvalsCode(codeVuln(input),v)));
+        forall v | v in vulnBehaviors
+            ensures !MiniSpec(v) ==> (behaviorOutput(v) == [Nil,Nil,Nil,Out((Int(1,IntType(1,false)))),Out((Int(1,IntType(1,false))))]);
+        {
+            assert (exists input :: ( validInput(s,input) && BehaviorEvalsCode(codeVuln(input),v)));
+            possibleVulnOutputsWithMiniSpec(s,v);
+            assert (!MiniSpec(v) ==>  (exists input :: (validInput(s,input) && OperandContents(s,input).val < 2 && BehaviorEvalsCode(codeVuln(input),v))));
+            assert !MiniSpec(v) ==> (behaviorOutput(v) == [Nil,Nil,Nil,Out((Int(1,IntType(1,false)))),Out((Int(1,IntType(1,false))))]);
+        } 
+
+
+        forall p | behaviorOutput(p) in vulnOut
+             ensures !MiniSpec(p) ==> behaviorOutput(p) in vulnOut;
+        {
+            if (MiniSpec(p)){
+                assert behaviorOutput(p) in vulnOut;
+            }else{
+                assert !MiniSpec(p);
+                assert behaviorOutput(p) in vulnOut;
+            }
+        }
+
+        assert forall p :: constrainedBehavorSet(p,vulnOut) ==> behaviorInAll(behaviorOutput(p),vulnOut);// behaviorOutput(p) in vulnOut;
+        assert forall p :: behaviorInAll(behaviorOutput(p),vulnOut) ==> existsSameOutput(vulnBehaviors,p);//(exists p' :: p' in vulnBehaviors && behaviorOutput(p) == behaviorOutput(p'));
+        assert forall p :: constrainedBehavorSet(p,vulnOut) ==> existsSameOutput(vulnBehaviors,p);//(exists p' :: p' in vulnBehaviors && behaviorOutput(p) == behaviorOutput(p'));
+
+    }
+
+    predicate  existsSameOutput(vulnBehaviors:seq<behavior>,p:behavior)
+    {
+        exists p' :: p' in vulnBehaviors && behaviorOutput(p) == behaviorOutput(p')
+    }
+
+    predicate existsSameOutputConstrained(vulnBehaviors:seq<behavior>,p:behavior)
+    {
+        exists p' :: p' in vulnBehaviors && !MiniSpec(p') && behaviorOutput(p) == behaviorOutput(p')
+    }
+    predicate behaviorInAll(out:seq<output>,vulnOut:seq<seq<output>>)
+    {
+        out in vulnOut
+    }
+
+    predicate constrainedBehavorSet(b:behavior,vulnOut:seq<seq<output>>)
+    {
+        behaviorOutput(b) in vulnOut && !MiniSpec(b)
+    }
+
+    lemma patchIsCompleteTrivial(s:state,vulnBehaviors:seq<behavior>,patchBehaviors:seq<behavior>,vulnOut:seq<seq<output>>,patchOut:seq<seq<output>>)
+        requires |vulnBehaviors| == 0
+        requires |vulnOut| == 0
+        requires ValidState(s);
+        requires forall b :: b in vulnBehaviors <==> (exists input :: validInput(s,input) &&  ValidBehaviorNonTrivial(b) && BehaviorEvalsCode(codeVuln(input),b) && b[0] == s)
+        requires forall b :: b in patchBehaviors <==> (exists input :: validInput(s,input) &&  ValidBehaviorNonTrivial(b) && BehaviorEvalsCode(codePatch(input),b) && b[0] == s)
+
+        ensures forall p :: (behaviorOutput(p) in vulnOut && !MiniSpec(p))  ==> behaviorOutput(p) in patchOut
+        {
+           
+            assert |vulnBehaviors| == 0;
+            assert |vulnOut| == 0;
+            assert forall p :: (behaviorOutput(p) in vulnOut && !MiniSpec(p))  ==> behaviorOutput(p) in patchOut;
+            
+        }
+
+    lemma patchIsCompleteNonTrivial(s:state,vulnBehaviors:seq<behavior>,patchBehaviors:seq<behavior>,vulnOut:seq<seq<output>>,patchOut:seq<seq<output>>)
+        requires nonTrivialBehaviorPreconditions(s,vulnBehaviors,patchBehaviors)
+        requires |vulnBehaviors| > 0
+        requires ValidState(s);
+                    
+        requires |patchBehaviors| > 0;
+
+        requires vulnOut == allBehaviorOutput(vulnBehaviors);
+        requires patchOut ==  allBehaviorOutput(patchBehaviors);
+
+        ensures forall p :: p in vulnBehaviors && !MiniSpec(p) ==> (behaviorOutput(p) in vulnOut && behaviorOutput(p) in patchOut);
+        // ensures forall p :: (behaviorOutput(p) in vulnOut && !MiniSpec(p))  ==> behaviorOutput(p) in patchOut
+        // ensures forall p :: p in (reducedVulnModMS(s,vulnBehaviors,patchBehaviors,vulnOut)) ==> p in patchOut;
+        {
+            reveal_BehaviorEvalsCode();
+            
+            reveal_nonTrivialBehaviorPreconditionsVuln();
+            reveal_nonTrivialBehaviorPreconditionsPatch();
+            
+            
+            forall p | (p in vulnBehaviors && !MiniSpec(p))
+                ensures equalOutput(behaviorOutput(p),[Nil,Nil,Nil,Out((Int(1,IntType(1,false)))),Out((Int(1,IntType(1,false))))]);
+                ensures behaviorOutput(p) in vulnOut;
+                ensures behaviorOutput(p) in patchOut;
+            {
+                var input :| BehaviorEvalsCode(codeVuln(input),p) && |p| > 0 && validInput(p[0],input);
+                var b' := unwrapVulnBehaviors(s,input);
+                possibleVulnOutputsWithMiniSpec(s,p);
+                assert equalOutput(behaviorOutput(p),[Nil,Nil,Nil,Out((Int(1,IntType(1,false)))),Out((Int(1,IntType(1,false))))]);
+                assert behaviorOutput(p) in vulnOut;
+
+                var singlePatchBehavior :| singlePatchBehavior in patchBehaviors;
+                var patchInput :| BehaviorEvalsCode(codePatch(patchInput),singlePatchBehavior) && |singlePatchBehavior| > 0 && validInput(singlePatchBehavior[0],patchInput);
+                var patch' := unwrapPatchBehaviors(s,patchInput);
+                outputIsEqual(behaviorOutput(patch'),[Nil,Nil,Nil,Out((Int(1,IntType(1,false)))),Out((Int(1,IntType(1,false))))]);
+                assert equalOutput(behaviorOutput(patch'),[Nil,Nil,Nil,Out((Int(1,IntType(1,false)))),Out((Int(1,IntType(1,false))))]);
+                assert behaviorOutput(patch') in patchOut;
+                transitiveEquality(behaviorOutput(patch'),behaviorOutput(p),[Nil,Nil,Nil,Out((Int(1,IntType(1,false)))),Out((Int(1,IntType(1,false))))]);
+                equalOutputIsTransitive(behaviorOutput(patch'),behaviorOutput(p),patchOut);
+
+            }
+             forall p | p in patchBehaviors
+                ensures equalOutput(behaviorOutput(p),[Nil,Nil,Nil,Out((Int(1,IntType(1,false)))),Out((Int(1,IntType(1,false))))]);
+                ensures behaviorOutput(p) in patchOut;
+             {
+                var input :| BehaviorEvalsCode(codePatch(input),p) && |p| > 0 && validInput(p[0],input);
+                var b' := unwrapPatchBehaviors(s,input);
+                assert equalOutput(behaviorOutput(p),[Nil,Nil,Nil,Out((Int(1,IntType(1,false)))),Out((Int(1,IntType(1,false))))]);
+                assert behaviorOutput(p) in patchOut;
+
+             }
+
+            allOutputConstrainedImpliesSameBehaviorOExists(s,vulnBehaviors,patchBehaviors,vulnOut);
+            assert forall p :: constrainedBehavorSet(p,vulnOut) ==> existsSameOutput(vulnBehaviors,p);
+            var reduced := reducedVulnModMS(s,vulnBehaviors,patchBehaviors,vulnOut);
+
+            // forall p :: (behaviorOutput(p) in aOut && !MiniSpec(p)) ==> behaviorOutput(p) in bOut
+            // assert forall p :: p in reduced ==> (equalOutput(p,[Nil,Nil,Nil,Out((Int(0,IntType(1,false)))),Out((Int(0,IntType(1,false))))])); 
+            assert forall p :: p in reduced ==> equalOutput(p,[Nil,Nil,Nil,Out((Int(1,IntType(1,false)))),Out((Int(1,IntType(1,false))))]);
+            // assert forall p :: p in patchOut ==> equalOutput(p,[Nil,Nil,Nil,Out((Int(1,IntType(1,false)))),Out((Int(1,IntType(1,false))))]);
+            forall p | p in reduced
+                ensures p in patchOut;
+            {
+                assert equalOutput(p,[Nil,Nil,Nil,Out((Int(1,IntType(1,false)))),Out((Int(1,IntType(1,false))))]);
+                assert exists b :: b in patchOut && equalOutput(b,[Nil,Nil,Nil,Out((Int(1,IntType(1,false)))),Out((Int(1,IntType(1,false))))]);
+                var b :| b in patchOut && equalOutput(b,[Nil,Nil,Nil,Out((Int(1,IntType(1,false)))),Out((Int(1,IntType(1,false))))]);
+                assert b == p;
+                assert p in patchOut;
+            }
+            assert forall p :: p in reduced ==> p in patchOut;
+
+        }
+
+            // assert (forall b :: behaviorOutput(b) in vulnOut <==> (exists input :: validInput(s,input) &&  ValidBehaviorNonTrivial(b) && BehaviorEvalsCode(codeVuln(input),b) && b[0] == s));
+
+    lemma reducedVulnModMS(s:state,vulnBehaviors:seq<behavior>,patchBehaviors:seq<behavior>,vulnOut:seq<seq<output>>) returns (moduloMSOut:seq<seq<output>>)
+            requires nonTrivialBehaviorPreconditions(s,vulnBehaviors,patchBehaviors)
+            requires vulnOut == allBehaviorOutput(vulnBehaviors);
+            requires forall p :: constrainedBehavorSet(p,vulnOut) ==> existsSameOutput(vulnBehaviors,p);
+            ensures forall reducedP :: reducedP in moduloMSOut ==> equalOutput(reducedP,[Nil,Nil,Nil,Out((Int(1,IntType(1,false)))),Out((Int(1,IntType(1,false))))]);
+
+    {
+        reveal_nonTrivialBehaviorPreconditionsVuln();
+        reveal_nonTrivialBehaviorPreconditionsPatch();
+        assert (forall b :: b in vulnBehaviors <==> (exists input :: validInput(s,input) &&  ValidBehaviorNonTrivial(b) && BehaviorEvalsCode(codeVuln(input),b) && b[0] == s));
+        assert forall i :: (i >= 0 && i < |vulnBehaviors|) ==> vulnOut[i] == behaviorOutput(vulnBehaviors[i]);
+        var moduloMs :| vulnModMiniSpec(s,vulnBehaviors,moduloMs);
+        // assert nonTrivialBehaviorPreconditionsVuln(s,test);
+        assert forall p :: p in moduloMs ==> !MiniSpec(p);
+        var reducedOut := allBehaviorOutput(moduloMs);
+        forall p | p in moduloMs
+            ensures equalOutput(behaviorOutput(p),[Nil,Nil,Nil,Out((Int(1,IntType(1,false)))),Out((Int(1,IntType(1,false))))]);
+            ensures behaviorOutput(p) in reducedOut;
+        {
+            possibleVulnOutputsWithMiniSpec(s,p);
+            assert equalOutput(behaviorOutput(p),[Nil,Nil,Nil,Out((Int(1,IntType(1,false)))),Out((Int(1,IntType(1,false))))]);
+            assert behaviorOutput(p) in reducedOut;
+        }
+        assert forall reducedP :: reducedP in reducedOut ==> equalOutput(reducedP,[Nil,Nil,Nil,Out((Int(1,IntType(1,false)))),Out((Int(1,IntType(1,false))))]);
+        moduloMSOut := reducedOut;
+    }
+
+    predicate vulnModMiniSpec(s:state,vulnBehaviors:seq<behavior>,vulnBehaviorsConstrained:seq<behavior> ) //: vulnBehaviorsConstrained:seq<behavior> 
+        requires ValidState(s);
+        requires nonTrivialBehaviorPreconditionsVuln(s,vulnBehaviors)
+        {
+            && (forall p :: p in vulnBehaviorsConstrained ==> (!MiniSpec(p) && p in vulnBehaviors))
+            && (forall b :: b in vulnBehaviorsConstrained ==> (exists input :: validInput(s,input) &&  ValidBehaviorNonTrivial(b) && BehaviorEvalsCode(codeVuln(input),b) && b[0] == s))
+
+        }
+////
+
+lemma makeConnection(s:state,vulnBehaviors:seq<behavior>,patchBehaviors:seq<behavior>,vulnOut:seq<seq<output>>)
+            requires nonTrivialBehaviorPreconditions(s,vulnBehaviors,patchBehaviors)
+            requires vulnOut == allBehaviorOutput(vulnBehaviors);
+            requires forall p :: constrainedBehavorSet(p,vulnOut) ==> existsSameOutput(vulnBehaviors,p);
+            // requires forall p :: p in vulnBehaviors ==> (equalOutput(behaviorOutput(p),[Nil,Nil,Nil,Out((Int(0,IntType(1,false)))),Out((Int(0,IntType(1,false))))]) 
+            //                 || equalOutput(behaviorOutput(p),[Nil,Nil,Nil,Out((Int(1,IntType(1,false)))),Out((Int(1,IntType(1,false))))])); 
+            requires forall p :: p in vulnBehaviors ==> (!MiniSpec(p) <==> equalOutput(behaviorOutput(p),[Nil,Nil,Nil,Out((Int(1,IntType(1,false)))),Out((Int(1,IntType(1,false))))]));
+    {
+            reveal_nonTrivialBehaviorPreconditionsVuln();
+            reveal_nonTrivialBehaviorPreconditionsPatch();
+            reveal_behaviorOutput();
+
+            forall p | constrainedBehavorSet(p,vulnOut)
+                {
+                    var p' :| p' in vulnBehaviors && behaviorOutput(p) == behaviorOutput(p');
+                    possibleVulnOutputs(s,p');
+                    possibleVulnOutputsWithMiniSpec(s,p');
+                    assert (equalOutput(behaviorOutput(p'),[Nil,Nil,Nil,Out((Int(0,IntType(1,false)))),Out((Int(0,IntType(1,false))))]) 
+                            || equalOutput(behaviorOutput(p'),[Nil,Nil,Nil,Out((Int(1,IntType(1,false)))),Out((Int(1,IntType(1,false))))]));
+                    assert (equalOutput(behaviorOutput(p),[Nil,Nil,Nil,Out((Int(0,IntType(1,false)))),Out((Int(0,IntType(1,false))))]) 
+                            || equalOutput(behaviorOutput(p),[Nil,Nil,Nil,Out((Int(1,IntType(1,false)))),Out((Int(1,IntType(1,false))))]));
+                    // assert !MiniSpec(p');
+                    assert !MiniSpec(p);
+                    assert MiniSpec(p') <==> equalOutput(behaviorOutput(p'),[Nil,Nil,Nil,Out((Int(0,IntType(1,false)))),Out((Int(0,IntType(1,false))))]);
+                    assert MiniSpec(p') ==> equalOutput(behaviorOutput(p),[Nil,Nil,Nil,Out((Int(0,IntType(1,false)))),Out((Int(0,IntType(1,false))))]);
+                    assert !MiniSpec(p') ==> equalOutput(behaviorOutput(p),[Nil,Nil,Nil,Out((Int(1,IntType(1,false)))),Out((Int(1,IntType(1,false))))]);
+
+                    // possibleVulnOutputsWithMiniSpec(s,p);
+                    // assert MiniSpec(p) <==> equalOutput(behaviorOutput(p),[Nil,Nil,Nil,Out((Int(0,IntType(1,false)))),Out((Int(0,IntType(1,false))))]);
+                }
+    }
+
+    ////
+    // function vulnModMiniSpecCreate(s:state,vulnBehaviors:seq<behavior>) : (vulnBehaviorsConst:seq<behavior>)
+    //     requires ValidState(s);
+    //     requires nonTrivialBehaviorPreconditionsVuln(s,vulnBehaviors)
+    //     decreases |vulnBehaviors|
+    //     {
+    //         reveal_nonTrivialBehaviorPreconditionsVuln();
+    //         if |vulnBehaviors| == 0 then
+    //             []
+    //         else
+    //             if !MiniSpec(vulnBehaviors[0]) then
+    //                    assert (forall b :: b in all_but_first(vulnBehaviors) ==> (exists input :: validInput(s,input) &&  ValidBehaviorNonTrivial(b) && BehaviorEvalsCode(codeVuln(input),b) && b[0] == s));
+
+    //                 assert nonTrivialBehaviorPreconditionsVuln(s,all_but_first(vulnBehaviors));
+    //                 var out := [vulnBehaviors[0]] + vulnModMiniSpecCreate(s,all_but_first(vulnBehaviors));
+    //                 out
+    //             else
+    //                 vulnModMiniSpecCreate(s,all_but_first(vulnBehaviors))
+    //             // out
+
+    //     }
+
+    // function allBehaviorOutputVuln(s:state,a:seq<behavior>) : (bOut:seq<seq<output>>)
+    //     requires ValidState(s);
+    //     // requires nonTrivialBehaviorPreconditionsVuln(s,a)
+    //     requires (forall b :: b in a ==> (exists input :: validInput(s,input) &&  ValidBehaviorNonTrivial(b) && BehaviorEvalsCode(codeVuln(input),b) && b[0] == s))
+
+    //     ensures |bOut| == |a|
+    //     ensures forall a' :: a' in a ==> behaviorOutput(a') in bOut;
+    //     ensures forall i :: (i >= 0 && i < |a|) ==> bOut[i] == behaviorOutput(a[i])
+    //     ensures |a| == 0 ==> |bOut| == 0;
+    //     //  ensures forall i :: (i >= 0 && i < |a|) ==> (exists input :: validInput(s,input) &&  ValidBehaviorNonTrivial(b) && BehaviorEvalsCode(codeVuln(input),b) && b[0] == s))
+    //     // ensures forall i :: (i >= 0 && i < |a|) ==> (bOut[i] == behaviorOutput(a[i])
+    //     //                                             && (exists input :: validInput(s,input) &&  ValidBehaviorNonTrivial(a[i]) && BehaviorEvalsCode(codeVuln(input),a[i]) && a[i][0] == s))
+    //     // ensures forall b :: behaviorOutput(b) in bOut ==> (exists a' :: a' in a && behaviorOutput(b) == behaviorOutput(a')); 
+    //     ensures forall b :: behaviorOutput(b) in bOut ==> (exists b' :: b' in a && behaviorOutput(b) == behaviorOutput(b'));
+        
+    //     decreases |a|
+    // {
+    //     reveal_nonTrivialBehaviorPreconditionsVuln();
+    //     // assert 
+    //     if |a| == 0 then
+    //         var out := [];
+    //         // assert forall a' :: behaviorOutput(a') in out ==> a' in a;
+    //         out
+    //     else   
+    //         var subset := all_but_first(a);
+    //         if |subset| == 0 then
+    //             var out := [behaviorOutput(a[0])];
+    //             out
+    //         else
+    //             subsetProperty(s,subset);
+    //             var out := [behaviorOutput(a[0])] + allBehaviorOutputVuln(s,subset);
+    //             out
+    // }
+
+    // lemma subsetProperty(s:state,a:seq<behavior>)
+    //     requires ValidState(s);
+    //     requires |a| > 0
+    //     requires (forall b :: b in a ==> (exists input :: validInput(s,input) &&  ValidBehaviorNonTrivial(b) && BehaviorEvalsCode(codeVuln(input),b) && b[0] == s))
+    //     ensures (forall b :: b in all_but_first(a) ==> (exists input :: validInput(s,input) &&  ValidBehaviorNonTrivial(b) && BehaviorEvalsCode(codeVuln(input),b) && b[0] == s));
+
+    // {
+    //    var subset := all_but_first(a);
+    //    assert (forall b :: b in subset ==> (exists input :: validInput(s,input) &&  ValidBehaviorNonTrivial(b) && BehaviorEvalsCode(codeVuln(input),b) && b[0] == s));
+            
+    // }
+
+
+    /// OLD
+
+
+            // forall p | p in vulnBehaviors
+            //     ensures (equalOutput(behaviorOutput(p),[Nil,Nil,Nil,Out((Int(0,IntType(1,false)))),Out((Int(0,IntType(1,false))))]) 
+            //                 || equalOutput(behaviorOutput(p),[Nil,Nil,Nil,Out((Int(1,IntType(1,false)))),Out((Int(1,IntType(1,false))))]));                
+            //     ensures !MiniSpec(p) <==> equalOutput(behaviorOutput(p),[Nil,Nil,Nil,Out((Int(1,IntType(1,false)))),Out((Int(1,IntType(1,false))))]);
+            //     ensures behaviorOutput(p) in vulnOut;
+            //  {
+            //     var input :| BehaviorEvalsCode(codeVuln(input),p) && |p| > 0 && validInput(p[0],input);
+            //     var b' := unwrapVulnBehaviors(s,input);
+            //     possibleVulnOutputs(s,b');
+            //     possibleVulnOutputsWithMiniSpec(s,b');
+            //     assert !MiniSpec(b') <==> equalOutput(behaviorOutput(b'),[Nil,Nil,Nil,Out((Int(1,IntType(1,false)))),Out((Int(1,IntType(1,false))))]);
+            //     assert (equalOutput(behaviorOutput(b'),[Nil,Nil,Nil,Out((Int(0,IntType(1,false)))),Out((Int(0,IntType(1,false))))]) 
+            //                 || equalOutput(behaviorOutput(b'),[Nil,Nil,Nil,Out((Int(1,IntType(1,false)))),Out((Int(1,IntType(1,false))))]));                
+            //     // assert equalOutput(behaviorOutput(p),[Nil,Nil,Nil,Out((Int(1,IntType(1,false)))),Out((Int(1,IntType(1,false))))]);
+            //     // assert behaviorOutput(p) in patchOut;
+            //     assert behaviorOutput(p) in vulnOut;
+
+            //  }
+            // assert forall p :: p in vulnOut ==> equalOutput(p,[Nil,Nil,Nil,Out((Int(0,IntType(1,false)))),Out((Int(0,IntType(1,false))))]) || equalOutput(p,[Nil,Nil,Nil,Out((Int(1,IntType(1,false)))),Out((Int(1,IntType(1,false))))]);
+
+            // assert forall p :: p in patchOut ==> equalOutput(p,[Nil,Nil,Nil,Out((Int(1,IntType(1,false)))),Out((Int(1,IntType(1,false))))]);
+            // assert forall p :: behaviorOutput(p) in patchOut ==> equalOutput(behaviorOutput(p),[Nil,Nil,Nil,Out((Int(1,IntType(1,false)))),Out((Int(1,IntType(1,false))))]);
+            
+            // var p' :| 
+            // assert forall i :: (i >= 0 && i < |vulnOut|) ==> vulnOut[i] == behaviorOutput(vulnBehaviors[i]);
+            // assert forall v :: (v in vulnBehaviors && !MiniSpec(v)) ==> 
+            //             ((behaviorOutput(v) == [Nil,Nil,Nil,Out((Int(1,IntType(1,false)))),Out((Int(1,IntType(1,false))))]));
+            // assert forall p :: constrainedBehavorSet(p,vulnOut) ==> (equalOutput(behaviorOutput(p),[Nil,Nil,Nil,Out((Int(0,IntType(1,false)))),Out((Int(0,IntType(1,false))))]) 
+            //                 || equalOutput(behaviorOutput(p),[Nil,Nil,Nil,Out((Int(1,IntType(1,false)))),Out((Int(1,IntType(1,false))))])); 
+            // assert forall p :: constrainedBehavorSet(p,vulnOut) ==> !MiniSpec(p); 
+
+            // forall p | constrainedBehavorSet(p,vulnOut)
+            // {
+            //     var p' :| p' in vulnBehaviors && behaviorOutput(p) == behaviorOutput(p');
+            // }
+            // assert forall p :: constrainedBehavorSet(p,vulnOut) ==> equalOutput(behaviorOutput(p),[Nil,Nil,Nil,Out((Int(1,IntType(1,false)))),Out((Int(1,IntType(1,false))))]);
+                    
+                    //   assert forall p :: constrainedBehavorSet(p,vulnOut) ==> existsSameOutputConstrained(vulnBehaviors,p);
+
+            // assert forall p :: constrainedBehavorSet(p,vulnOut)==> ((behaviorOutput(p) == [Nil,Nil,Nil,Out((Int(1,IntType(1,false)))),Out((Int(1,IntType(1,false))))]));
+            // assert forall i :: (i >= 0 && i < |vulnOut|) ==> (!MiniSpec(vulnBehaviors[i]) ==>  equalOutput(vulnOut[i],[Nil,Nil,Nil,Out((Int(1,IntType(1,false)))),Out((Int(1,IntType(1,false))))] ));
+            
+            // assert (forall p :: behaviorOutput(p) in vulnOut ==> (exists input :: validInput(s,input) && BehaviorEvalsCode(codeVuln(input),p)));
+            // assert forall p :: (p in vulnBehaviors && !MiniSpec(p)) ==> equalOutput(behaviorOutput(p),[Nil,Nil,Nil,Out((Int(1,IntType(1,false)))),Out((Int(1,IntType(1,false))))] );
+            
+
+
+
+
+}
