Dafny/examples/BasicBug/simpleBugGeneral.i.dfy
@@ -6,6 +6,7 @@ module simpleBugGeneral{
     import opened LLVM_defRE
     import opened types
     import opened Collections__Seqs_s
+    import opened Collections__Sets_i
 
         // benignPatch: "The patch does not add any NEW behaviors"
     predicate benignPatch(a:seq<behavior>,b:seq<behavior>)
@@ -14,6 +15,22 @@ module simpleBugGeneral{
         var bOut := allBehaviorOutput(b);
         forall p :: p in bOut ==> p in aOut
 
+    }
+
+  // successfulPatch: "The patch prunes the BAD (defined by MiniSpec) behaviors"
+    predicate successfulPatch(b:seq<behavior>)
+    {
+        forall p :: MiniSpec(p) ==> !(p in b)
+    }
+
+    // completePatch: "The patch preserves the GOOD behavior" // Name; complete -> preserving ? 
+    predicate completePatch(a:seq<behavior>,b:seq<behavior>)
+    {
+        // forall p :: (p in a && !MiniSpec(p)) ==> p in b
+
+        var aOut := allBehaviorOutput(a);
+        var bOut := allBehaviorOutput(b);
+        forall p :: (behaviorOutput(p) in aOut && !MiniSpec(p)) ==> behaviorOutput(p) in bOut
     }
 
 
@@ -38,11 +55,7 @@ module simpleBugGeneral{
         RemovedBehaviors(b)
     }
 
-    // successfulPatch: "The patch prunes the BAD (defined by MiniSpec) behaviors"
-    predicate successfulPatch(b:seq<behavior>)
-    {
-        forall p :: MiniSpec(p) ==> !(p in b)
-    }
+  
 
 
     
