Dafny/examples/BasicBug/simpleBugProperties.i.dfy
@@ -1,4 +1,5 @@
 include "simpleBugBenignLemmas.i.dfy"
+include "simpleBugCompleteLemmas.i.dfy"
 include "simpleBugCode.i.dfy"
 include "../../LLVM/llvmREFACTOR.i.dfy"
 include "../../LLVM/types.dfy"
@@ -8,6 +9,7 @@ include "../../Libraries/Seqs.s.dfy"
 
 module simpleBugProperties{
     import opened simpleBugBenignLemmas
+    import opened simpleBugCompleteLemmas
     import opened simpleBugCode
     import opened LLVM_defRE
     import opened types
@@ -26,6 +28,9 @@ module simpleBugProperties{
         requires nonTrivialBehaviorPreconditions(s,vulnBehaviors,patchBehaviors)
         ensures benignPatch(vulnBehaviors,patchBehaviors)
     {
+        reveal_nonTrivialBehaviorPreconditionsVuln();
+        reveal_nonTrivialBehaviorPreconditionsPatch();
+        
         var vulnOut := allBehaviorOutput(vulnBehaviors);
         var patchOut :=  allBehaviorOutput(patchBehaviors);
         if (|patchBehaviors| == 0){
@@ -44,11 +49,14 @@ module simpleBugProperties{
 //         forall p :: MiniSpec(p) ==> !(p in b)
 //     }
 
- lemma patchIssuccessful(s:state,patchBehaviors:seq<behavior>)
+ lemma patchIsSuccessful(s:state,patchBehaviors:seq<behavior>)
         requires ValidState(s);
         requires nonTrivialBehaviorPreconditionsPatch(s,patchBehaviors)
         ensures successfulPatch(patchBehaviors)
     {    
+        reveal_nonTrivialBehaviorPreconditionsVuln();
+        reveal_nonTrivialBehaviorPreconditionsPatch();
+        
         var result := LV("result");
          if (|patchBehaviors| == 0){
              assert forall p :: MiniSpec(p) ==> !(p in patchBehaviors);
@@ -68,6 +76,31 @@ module simpleBugProperties{
                 assert forall p :: MiniSpec(p) ==> !(p in patchBehaviors);
              }
          }
+    
+    // forall p :: (behaviorOutput(p) in aOut && !MiniSpec(p)) ==> behaviorOutput(p) in bOut
+    lemma patchIsComplete(s:state,vulnBehaviors:seq<behavior>,patchBehaviors:seq<behavior>)
+        requires ValidState(s);
+        requires nonTrivialBehaviorPreconditions(s,vulnBehaviors,patchBehaviors)
+        // ensures completePatch(vulnBehaviors,patchBehaviors)
+    {
+        reveal_nonTrivialBehaviorPreconditionsVuln();
+        reveal_nonTrivialBehaviorPreconditionsPatch();
+        reveal_behaviorOutput();
+        // reveal_BehaviorEvalsCode();
+        var vulnOut := allBehaviorOutput(vulnBehaviors);
+        var patchOut :=  allBehaviorOutput(patchBehaviors);
+        // assert forall p :: behaviorOutput(p) in vulnOut <==> (exists i :: (i >= 0 && i < |vulnBehaviors|) && vulnOut[i] == behaviorOutput(vulnBehaviors[i]));
+        if(|vulnBehaviors| == 0){
+            patchIsCompleteTrivial(s,vulnBehaviors,patchBehaviors,vulnOut,patchOut);
+            assert (forall p :: (behaviorOutput(p) in vulnOut && !MiniSpec(p))  ==> behaviorOutput(p) in patchOut);
+
+        }
+         if (|patchBehaviors| > 0){
+            patchIsCompleteNonTrivial(s,vulnBehaviors,patchBehaviors,vulnOut,patchOut);
+            // assert (forall p :: (p in vulnBehaviors && !MiniSpec(p)) ==> p in patchBehaviors);
+            // assert (forall p :: (behaviorOutput(p) in vulnOut && !MiniSpec(p))  ==> behaviorOutput(p) in patchOut);
+         }
+    }
     
 
 }
