Dafny/examples/BasicBugSet/simpleBugCompleteLemmasV2.i.dfy
@@ -1,0 +1,330 @@
+include "simpleBugCode.i.dfy"
+include "simpleBugGeneral.i.dfy"
+include "../../LLVM/llvmREFACTOR.i.dfy"
+include "../../LLVM/types.dfy"
+include "../../Libraries/Seqs.s.dfy"
+include "../../Libraries/Sets.i.dfy"
+
+module simpleBugCompleteLemmasV2{
+    import opened simpleBugCode
+    import opened simpleBugGeneral
+    import opened LLVM_defRE
+    import opened types
+    import opened Collections__Seqs_s
+    import opened Collections__Sets_i
+
+lemma possibleVulnOutputs(s:state, b:behavior) 
+        requires ValidState(s);
+        requires |b| > 0;
+        requires b[0] == s;
+        requires s.o.Nil?;
+
+        ensures  forall input :: (validInput(s,input) && OperandContents(s,input).val < 2 && BehaviorEvalsCode(codeVuln(input),b)) 
+                                  ==> (behaviorOutput(b) == [Nil,Nil,Nil,Out((Int(1,IntType(1,false)))),Out((Int(1,IntType(1,false))))]);
+        ensures  forall input :: (validInput(s,input) && OperandContents(s,input).val >= 2 && BehaviorEvalsCode(codeVuln(input),b)) 
+                                  ==> (behaviorOutput(b) == [Nil,Nil,Nil,Out((Int(0,IntType(1,false)))),Out((Int(0,IntType(1,false))))]);
+    {
+        var inputWitness := D(Int(1,IntType(4,false)));
+        assert validInput(s,inputWitness);
+        forall input | validInput(s,input) && OperandContents(s,input).val < 2 && BehaviorEvalsCode(codeVuln(input),b)
+            ensures (behaviorOutput(b) == [Nil,Nil,Nil,Out((Int(1,IntType(1,false)))),Out((Int(1,IntType(1,false))))]);
+        {
+            var input :| validInput(s,input) && OperandContents(s,input).val < 2 && BehaviorEvalsCode(codeVuln(input),b);
+            var b' := unwrapVulnBehaviors(s,input);
+            behaviorThatEvalsSameCodeWithSameInitIsEqual(s,codeVuln(input),b');
+        }
+        forall input | validInput(s,input) && OperandContents(s,input).val >= 2 && BehaviorEvalsCode(codeVuln(input),b)
+            ensures (behaviorOutput(b) == [Nil,Nil,Nil,Out((Int(0,IntType(1,false)))),Out((Int(0,IntType(1,false))))]);
+        {
+            var input :| validInput(s,input) && OperandContents(s,input).val >= 2 && BehaviorEvalsCode(codeVuln(input),b);
+            var b' := unwrapVulnBehaviors(s,input);
+            behaviorThatEvalsSameCodeWithSameInitIsEqual(s,codeVuln(input),b');
+        }
+     
+    }
+
+    lemma possibleVulnOutputsWithMiniSpec(s:state, b:behavior)
+        requires ValidState(s);
+        requires |b| > 0;
+        requires b[0] == s;
+        requires s.o.Nil?;
+        ensures  forall input :: (validInput(s,input) && OperandContents(s,input).val < 2 && BehaviorEvalsCode(codeVuln(input),b)) 
+                                  ==> !MiniSpec(b);
+        ensures  forall input :: (validInput(s,input) && OperandContents(s,input).val >= 2 && BehaviorEvalsCode(codeVuln(input),b)) 
+                                  ==> MiniSpec(b);
+        ensures forall input :: ( validInput(s,input) && BehaviorEvalsCode(codeVuln(input),b)) ==> 
+                        (!MiniSpec(b) <==> (behaviorOutput(b) == [Nil,Nil,Nil,Out((Int(1,IntType(1,false)))),Out((Int(1,IntType(1,false))))]));
+         ensures forall input :: ( validInput(s,input) && BehaviorEvalsCode(codeVuln(input),b)) ==> 
+                        (MiniSpec(b) <==> (behaviorOutput(b) == [Nil,Nil,Nil,Out((Int(0,IntType(1,false)))),Out((Int(0,IntType(1,false))))]));
+    {
+        // possibleVulnOutputs(s,b);
+        var inputWitness := D(Int(1,IntType(4,false)));
+        assert validInput(s,inputWitness);
+        forall input | validInput(s,input) && OperandContents(s,input).val < 2 && BehaviorEvalsCode(codeVuln(input),b)
+            ensures !MiniSpec(b);
+            ensures (behaviorOutput(b) == [Nil,Nil,Nil,Out((Int(1,IntType(1,false)))),Out((Int(1,IntType(1,false))))]);
+            ensures !MiniSpec(b) ==> (behaviorOutput(b) == [Nil,Nil,Nil,Out((Int(1,IntType(1,false)))),Out((Int(1,IntType(1,false))))]);
+        {
+            var input :| validInput(s,input) && OperandContents(s,input).val < 2 && BehaviorEvalsCode(codeVuln(input),b);
+            var b' := unwrapVulnBehaviors(s,input);
+            behaviorThatEvalsSameCodeWithSameInitIsEqual(s,codeVuln(input),b');
+            assert !MiniSpec(b);
+            assert (behaviorOutput(b) == [Nil,Nil,Nil,Out((Int(1,IntType(1,false)))),Out((Int(1,IntType(1,false))))]);
+        }
+        forall input | validInput(s,input) && OperandContents(s,input).val >= 2 && BehaviorEvalsCode(codeVuln(input),b)
+            ensures MiniSpec(b);
+            ensures !(behaviorOutput(b) == [Nil,Nil,Nil,Out((Int(1,IntType(1,false)))),Out((Int(1,IntType(1,false))))]);
+            ensures MiniSpec(b) <==> (behaviorOutput(b) == [Nil,Nil,Nil,Out((Int(0,IntType(1,false)))),Out((Int(0,IntType(1,false))))]);
+        {
+            var input :| validInput(s,input) && OperandContents(s,input).val >= 2 && BehaviorEvalsCode(codeVuln(input),b);
+            var b' := unwrapVulnBehaviors(s,input);
+            behaviorThatEvalsSameCodeWithSameInitIsEqual(s,codeVuln(input),b');
+            assert MiniSpec(b);
+            assert (behaviorOutput(b) == [Nil,Nil,Nil,Out((Int(0,IntType(1,false)))),Out((Int(0,IntType(1,false))))]);
+            assert !(behaviorOutput(b) == [Nil,Nil,Nil,Out((Int(1,IntType(1,false)))),Out((Int(1,IntType(1,false))))]);
+        }
+        // assert !MiniSpec(b) ==> (behaviorOutput(b) == [Nil,Nil,Nil,Out((Int(1,IntType(1,false)))),Out((Int(1,IntType(1,false))))]);
+    }
+
+
+lemma findModMsSet(s:state,vulnBehaviors:set<behavior>) returns (vulnBehaviorsModMs:set<behavior>)
+    requires ValidState(s);
+    requires nonTrivialBehaviorPreconditionsVuln(s,vulnBehaviors);
+    ensures vulnBehaviorsModMs == MakeSubset(vulnBehaviors, x => !MiniSpec(x));
+    ensures forall p :: p in vulnBehaviorsModMs ==> !MiniSpec(p);
+    ensures nonTrivialBehaviorPreconditionsVulnModMs(s,vulnBehaviorsModMs);
+    // ensures (forall b :: b in vulnBehaviorsModMs ==> (exists input :: validInput(s,input) &&  ValidBehaviorNonTrivial(b) && BehaviorEvalsCode(codeVuln(input),b) && b[0] == s));
+{
+    reveal_nonTrivialBehaviorPreconditionsVuln();
+    reveal_nonTrivialBehaviorPreconditionsVulnModMs();
+    var subset := MakeSubset(vulnBehaviors, x => !MiniSpec(x));
+    forall v | v in subset
+        ensures (exists input :: validInput(s,input) &&  ValidBehaviorNonTrivial(v) && BehaviorEvalsCode(codeVuln(input),v) && v[0] == s);
+    {
+        assert v in vulnBehaviors;
+        assert (exists input :: validInput(s,input) &&  ValidBehaviorNonTrivial(v) && BehaviorEvalsCode(codeVuln(input),v) && v[0] == s);
+    }
+    vulnBehaviorsModMs := subset;
+
+}
+
+lemma vulnModMsOutput(s:state,vulnModMs:set<behavior>,vulnModMsOut:set<seq<output>>)
+        requires ValidState(s);
+        requires nonTrivialBehaviorPreconditionsVulnModMs(s,vulnModMs);
+        //requires (forall b :: b in vulnModMs ==> (exists input :: validInput(s,input) &&  ValidBehaviorNonTrivial(b) && BehaviorEvalsCode(codeVuln(input),b) && b[0] == s));
+        requires forall p :: p in vulnModMs ==> !MiniSpec(p);
+        requires vulnModMsOut == allBehaviorOutputSet(vulnModMs);
+        ensures forall b :: b in vulnModMsOut ==> equalOutput(b,[Nil,Nil,Nil,Out((Int(1,IntType(1,false)))),Out((Int(1,IntType(1,false))))]);
+    {
+        reveal_nonTrivialBehaviorPreconditionsVulnModMs();
+        forall p | p in vulnModMs
+            ensures (behaviorOutput(p) == [Nil,Nil,Nil,Out((Int(1,IntType(1,false)))),Out((Int(1,IntType(1,false))))]);
+        {
+            possibleVulnOutputsWithMiniSpec(s,p);
+            assert !MiniSpec(p);
+            assert (behaviorOutput(p) == [Nil,Nil,Nil,Out((Int(1,IntType(1,false)))),Out((Int(1,IntType(1,false))))]);
+        }
+        assert forall b :: b in vulnModMsOut ==> equalOutput(b,[Nil,Nil,Nil,Out((Int(1,IntType(1,false)))),Out((Int(1,IntType(1,false))))]);
+    }
+
+
+    lemma patchIsCompleteEmptyVulnSet(s:state,vulnModMs:set<behavior>,patchBehaviors:set<behavior>,vulnModMsOut:set<seq<output>>,patchOut:set<seq<output>>)
+        requires vulnModMsOut == allBehaviorOutputSet(vulnModMs);
+        requires patchOut ==  allBehaviorOutputSet(patchBehaviors);
+        requires |vulnModMs| == 0
+        requires |vulnModMsOut| == 0
+        requires ValidState(s);
+        requires nonTrivialBehaviorPreconditionsVulnModMs(s,vulnModMs);
+        // requires forall b :: b in vulnModMs ==> (exists input :: validInput(s,input) &&  ValidBehaviorNonTrivial(b) && BehaviorEvalsCode(codeVuln(input),b) && b[0] == s)
+        requires nonTrivialBehaviorPreconditionsPatch(s,patchBehaviors);
+
+        ensures forall p :: p in vulnModMsOut  ==> p in patchOut
+        {
+            reveal_nonTrivialBehaviorPreconditionsVulnModMs();
+            reveal_nonTrivialBehaviorPreconditionsPatch();
+            assert |vulnModMs| == 0;
+            assert |vulnModMsOut| == 0;
+            assert forall p :: p in vulnModMsOut  ==> p in patchOut;
+            
+        }
+
+    lemma patchIsCompleteNonTrivial(s:state,vulnModMs:set<behavior>,patchBehaviors:set<behavior>,vulnModMsOut:set<seq<output>>,patchOut:set<seq<output>>)
+        requires vulnModMsOut == allBehaviorOutputSet(vulnModMs);
+        requires patchOut ==  allBehaviorOutputSet(patchBehaviors);
+        requires |vulnModMs|  > 0
+        requires |patchBehaviors|  > 0
+        requires ValidState(s);
+        requires forall p :: p in vulnModMs ==> !MiniSpec(p);
+        requires nonTrivialBehaviorPreconditionsVulnModMs(s,vulnModMs);
+        // requires forall b :: b in vulnModMs ==> (exists input :: validInput(s,input) &&  ValidBehaviorNonTrivial(b) && BehaviorEvalsCode(codeVuln(input),b) && b[0] == s)
+        requires nonTrivialBehaviorPreconditionsPatch(s,patchBehaviors);
+        ensures forall p :: p in vulnModMsOut  ==> p in patchOut;
+    {
+        reveal_BehaviorEvalsCode();
+        reveal_nonTrivialBehaviorPreconditionsVuln();
+        reveal_nonTrivialBehaviorPreconditionsPatch();
+        reveal_nonTrivialBehaviorPreconditionsVulnModMs();
+
+                // reveal_evalCodeRE();
+                reveal_ValidBehavior();
+
+        vulnModMsOutput(s,vulnModMs,vulnModMsOut);
+        assert forall b :: b in vulnModMsOut ==> equalOutput(b,[Nil,Nil,Nil,Out((Int(1,IntType(1,false)))),Out((Int(1,IntType(1,false))))]);
+
+        forall p | p in patchBehaviors
+            ensures equalOutput(behaviorOutput(p),[Nil,Nil,Nil,Out((Int(1,IntType(1,false)))),Out((Int(1,IntType(1,false))))]);
+            ensures behaviorOutput(p) in patchOut;
+        {
+            var input :| BehaviorEvalsCode(codePatch(input),p) && |p| > 0 && validInput(p[0],input);
+            var b' := unwrapPatchBehaviors(s,input);
+            assert equalOutput(behaviorOutput(p),[Nil,Nil,Nil,Out((Int(1,IntType(1,false)))),Out((Int(1,IntType(1,false))))]);
+            assert behaviorOutput(p) in patchOut;
+        }
+
+        var patchB :| patchB in patchBehaviors;
+        var input :| BehaviorEvalsCode(codePatch(input),patchB) && |patchB| > 0 && validInput(patchB[0],input);
+        var b' := unwrapPatchBehaviors(s,input);
+        assert equalOutput(behaviorOutput(patchB),[Nil,Nil,Nil,Out((Int(1,IntType(1,false)))),Out((Int(1,IntType(1,false))))]);
+        assert behaviorOutput(patchB) in patchOut;
+
+        forall p | p in vulnModMsOut
+            ensures p in patchOut;
+        {
+            assert equalOutput(p,[Nil,Nil,Nil,Out((Int(1,IntType(1,false)))),Out((Int(1,IntType(1,false))))]);
+            transitiveEquality(p,behaviorOutput(patchB),[Nil,Nil,Nil,Out((Int(1,IntType(1,false)))),Out((Int(1,IntType(1,false))))]);
+            assert p == behaviorOutput(patchB);
+            equalOutputIsTransitiveSet(behaviorOutput(patchB),p,patchOut);
+            assert p in patchOut;
+        }
+        assert forall p :: p in vulnModMsOut  ==> p in patchOut;
+    }
+
+
+
+lemma patchBehaviorsInVulnModMSBehaviors(s:state,vulnModMs:set<behavior>,patchBehaviors:set<behavior>,vulnModMsOut:set<seq<output>>,patchOut:set<seq<output>>)
+        requires vulnModMsOut == allBehaviorOutputSet(vulnModMs);
+        requires patchOut ==  allBehaviorOutputSet(patchBehaviors);
+        requires |vulnModMs|  > 0
+        requires |patchBehaviors|  > 0
+        requires ValidState(s);
+        requires forall p :: p in vulnModMs ==> !MiniSpec(p);
+        requires nonTrivialBehaviorPreconditionsVulnModMs(s,vulnModMs);
+        requires nonTrivialBehaviorPreconditionsPatch(s,patchBehaviors);
+        // ensures forall p :: p in patchOut  ==> p in vulnModMsOut;
+        ensures forall p :: p in patchBehaviors ==> equalOutput(behaviorOutput(p),[Nil,Nil,Nil,Out((Int(1,IntType(1,false)))),Out((Int(1,IntType(1,false))))]);
+        ensures forall p :: p in patchBehaviors ==> behaviorOutput(p) in patchOut;
+        ensures forall p :: p in patchBehaviors ==> behaviorOutput(p) in vulnModMsOut;
+    {
+
+        reveal_BehaviorEvalsCode();
+        reveal_nonTrivialBehaviorPreconditionsVuln();
+        reveal_nonTrivialBehaviorPreconditionsPatch();
+        reveal_nonTrivialBehaviorPreconditionsVulnModMs();
+
+        vulnModMsOutput(s,vulnModMs,vulnModMsOut);
+        assert forall b :: b in vulnModMsOut ==> equalOutput(b,[Nil,Nil,Nil,Out((Int(1,IntType(1,false)))),Out((Int(1,IntType(1,false))))]);
+        assert |vulnModMsOut| > 0;
+        assert |patchBehaviors| > 0;
+        assert |patchOut| > 0;
+        var vulnMsBehaviorOut :| vulnMsBehaviorOut in vulnModMsOut;
+
+        forall p | p in patchBehaviors
+            ensures equalOutput(behaviorOutput(p),[Nil,Nil,Nil,Out((Int(1,IntType(1,false)))),Out((Int(1,IntType(1,false))))]);
+            ensures behaviorOutput(p) in patchOut;
+            ensures behaviorOutput(p) in vulnModMsOut;
+        {
+            var input :| BehaviorEvalsCode(codePatch(input),p) && |p| > 0 && validInput(p[0],input);
+            var b' := unwrapPatchBehaviors(s,input);
+            assert equalOutput(behaviorOutput(p),[Nil,Nil,Nil,Out((Int(1,IntType(1,false)))),Out((Int(1,IntType(1,false))))]);
+            assert behaviorOutput(p) in patchOut;
+            transitiveEquality(vulnMsBehaviorOut, behaviorOutput(p),[Nil,Nil,Nil,Out((Int(1,IntType(1,false)))),Out((Int(1,IntType(1,false))))]);
+            equalOutputIsTransitiveSet(vulnMsBehaviorOut,behaviorOutput(p),vulnModMsOut);
+            assert behaviorOutput(p) in vulnModMsOut;
+        }
+        // assert forall p :: p in patchBehaviors ==> behaviorOutput(p) in vulnModMsOut;
+        // allBehaviorEqualityIsInjective(patchBehaviors,patchOut); 
+        // allBehaviorsSetSurjective(patchBehaviors,patchOut);
+        // assert (forall y :: y in patchOut ==> (exists x :: x in patchBehaviors && behaviorOutput(x) == y));
+        // assert SurjectiveOver(patchBehaviors,patchOut, x => behaviorOutput(x));
+        // assert SurjectiveOver(patchBehaviors,patchOut, x => behaviorOutput(x)) ==> (forall y :: y in patchOut ==> (exists x :: x in patchBehaviors && behaviorOutput(x) == y));
+
+        // assert forall y :: y in test ==> (exists x :: x in patchBehaviors && behaviorOutput(x) == y);
+        // assert expandedAllBehaviorsSurjective(patchBehaviors,patchOut);// ==> (forall y :: y in patchOut ==> (exists x :: x in patchBehaviors && behaviorOutput(x) == y));
+        // assert  forall y :: y in patchOut ==> (exists x :: x in patchBehaviors && behaviorOutput(x) == y);
+        // forall pOut | behaviorOutput(pOut) in patchOut
+        // {
+        //     assert SurjectiveOver(patchBehaviors,patchOut, x => behaviorOutput(x));
+        //     // assert (exists p :: p in patchBehaviors && behaviorOutput(p) ==  behaviorOutput(pOut));
+        //     // assert equalOutput(behaviorOutput(pOut),[Nil,Nil,Nil,Out((Int(1,IntType(1,false)))),Out((Int(1,IntType(1,false))))]);
+        // }
+            //    assert  forall p :: p in patchOut  ==> p in vulnModMsOut;
+
+    }
+
+// lemma fullPatch(a:set<behavior>,b:set<behavior>)
+//     requires benignPatch(a,b);
+//     requires successfulPatch(b);
+//     requires completePatch(a,b);
+//     ensures safePatch(a,b);
+
+    // lemma patchIsCompleteNonTrivial(s:state,vulnBehaviors:set<behavior>,patchBehaviors:set<behavior>,vulnOut:set<seq<output>>,patchOut:set<seq<output>>)
+    //     requires nonTrivialBehaviorPreconditions(s,vulnBehaviors,patchBehaviors)
+    //     requires |vulnBehaviors| > 0
+    //     requires ValidState(s);
+                    
+    //     requires |patchBehaviors| > 0;
+
+    //     requires vulnOut == allBehaviorOutputSet(vulnBehaviors);
+    //     requires patchOut ==  allBehaviorOutputSet(patchBehaviors);
+
+    //     ensures forall p :: p in vulnBehaviors && !MiniSpec(p) ==> (behaviorOutput(p) in vulnOut && behaviorOutput(p) in patchOut);
+    //     // ensures forall p :: (behaviorOutput(p) in vulnOut && !MiniSpec(p))  ==> behaviorOutput(p) in patchOut
+    //     // ensures forall p :: p in (reducedVulnModMS(s,vulnBehaviors,patchBehaviors,vulnOut)) ==> p in patchOut;
+    //     {
+    //         reveal_BehaviorEvalsCode();
+            
+    //         reveal_nonTrivialBehaviorPreconditionsVuln();
+    //         reveal_nonTrivialBehaviorPreconditionsPatch();
+            
+            
+    //         forall p | (p in vulnBehaviors && !MiniSpec(p))
+    //             ensures equalOutput(behaviorOutput(p),[Nil,Nil,Nil,Out((Int(1,IntType(1,false)))),Out((Int(1,IntType(1,false))))]);
+    //             ensures behaviorOutput(p) in vulnOut;
+    //             ensures behaviorOutput(p) in patchOut;
+    //         {
+    //             var input :| BehaviorEvalsCode(codeVuln(input),p) && |p| > 0 && validInput(p[0],input);
+    //             var b' := unwrapVulnBehaviors(s,input);
+    //             possibleVulnOutputsWithMiniSpec(s,p);
+    //             assert equalOutput(behaviorOutput(p),[Nil,Nil,Nil,Out((Int(1,IntType(1,false)))),Out((Int(1,IntType(1,false))))]);
+    //             assert behaviorOutput(p) in vulnOut;
+
+    //             var singlePatchBehavior :| singlePatchBehavior in patchBehaviors;
+    //             var patchInput :| BehaviorEvalsCode(codePatch(patchInput),singlePatchBehavior) && |singlePatchBehavior| > 0 && validInput(singlePatchBehavior[0],patchInput);
+    //             var patch' := unwrapPatchBehaviors(s,patchInput);
+    //             outputIsEqual(behaviorOutput(patch'),[Nil,Nil,Nil,Out((Int(1,IntType(1,false)))),Out((Int(1,IntType(1,false))))]);
+    //             assert equalOutput(behaviorOutput(patch'),[Nil,Nil,Nil,Out((Int(1,IntType(1,false)))),Out((Int(1,IntType(1,false))))]);
+    //             assert behaviorOutput(patch') in patchOut;
+    //             transitiveEquality(behaviorOutput(patch'),behaviorOutput(p),[Nil,Nil,Nil,Out((Int(1,IntType(1,false)))),Out((Int(1,IntType(1,false))))]);
+    //             equalOutputIsTransitiveSet(behaviorOutput(patch'),behaviorOutput(p),patchOut);
+
+    //         }
+    //          forall p | p in patchBehaviors
+    //             ensures equalOutput(behaviorOutput(p),[Nil,Nil,Nil,Out((Int(1,IntType(1,false)))),Out((Int(1,IntType(1,false))))]);
+    //             ensures behaviorOutput(p) in patchOut;
+    //          {
+    //             var input :| BehaviorEvalsCode(codePatch(input),p) && |p| > 0 && validInput(p[0],input);
+    //             var b' := unwrapPatchBehaviors(s,input);
+    //             assert equalOutput(behaviorOutput(p),[Nil,Nil,Nil,Out((Int(1,IntType(1,false)))),Out((Int(1,IntType(1,false))))]);
+    //             assert behaviorOutput(p) in patchOut;
+
+    //          }
+
+    //     }
+
+            // assert (forall b :: behaviorOutput(b) in vulnOut <==> (exists input :: validInput(s,input) &&  ValidBehaviorNonTrivial(b) && BehaviorEvalsCode(codeVuln(input),b) && b[0] == s));
+
+
+
+
+
+}
