Dafny/examples/BasicBugSet/simpleBugGeneral.i.dfy
@@ -1,0 +1,105 @@
+include "../../LLVM/llvmREFACTOR.i.dfy"
+include "../../LLVM/types.dfy"
+include "../../Libraries/Seqs.s.dfy"
+include "../../Libraries/Sets.i.dfy"
+
+
+module simpleBugGeneral{
+    import opened LLVM_defRE
+    import opened types
+    import opened Collections__Seqs_s
+    import opened Collections__Sets_i
+
+        // benignPatch: "The patch does not add any NEW behaviors"
+    predicate benignPatch(a:set<behavior>,b:set<behavior>)
+    {
+        var aOut := allBehaviorOutputSet(a);
+        var bOut := allBehaviorOutputSet(b);
+        forall p :: p in bOut ==> p in aOut
+
+    }
+
+  // successfulPatch: "The patch prunes the BAD (defined by MiniSpec) behaviors"
+    predicate successfulPatch(b:set<behavior>)
+    {
+        forall p :: MiniSpec(p) ==> !(p in b)
+    }
+
+    // completePatch: "The patch preserves the GOOD behavior" // Name; complete -> preserving ? 
+    predicate completePatch(a:set<behavior>,b:set<behavior>)
+    {
+        // forall p :: (p in a && !MiniSpec(p)) ==> p in b
+
+        var aOut := allBehaviorOutputSet(a);
+        var bOut := allBehaviorOutputSet(b);
+        forall p :: (behaviorOutput(p) in aOut && !MiniSpec(p)) ==> behaviorOutput(p) in bOut
+    }
+    // completePatch: "The patch preserves the GOOD behavior" // Name; complete -> preserving ? 
+    predicate completePatchMS(a:set<behavior>,b:set<behavior>)
+    {
+        // forall p :: (p in a && !MiniSpec(p)) ==> p in b
+        var aModuloMS := MakeSubset(a, x => !MiniSpec(x));
+        var aOutMS := allBehaviorOutputSet(aModuloMS);
+        var bOut := allBehaviorOutputSet(b);
+        forall p :: behaviorOutput(p) in aOutMS ==> behaviorOutput(p) in bOut
+    }
+
+  predicate safePatch(a:set<behavior>,b:set<behavior>)
+    {
+        // forall p :: (p in a && !MiniSpec(p)) <==> p in b
+        var aOut := allBehaviorOutputSet(a);
+        var bOut := allBehaviorOutputSet(b);
+        forall p :: (behaviorOutput(p) in aOut && !MiniSpec(p)) <==> behaviorOutput(p) in bOut
+    }
+
+predicate safePatchMS(a:set<behavior>,b:set<behavior>)
+    {           
+    //  forall p :: (p in a && !MiniSpec(p)) <==> p in b
+        var aModuloMS := MakeSubset(a, x => !MiniSpec(x));
+        var aOutMS := allBehaviorOutputSet(aModuloMS);
+        var bOut := allBehaviorOutputSet(b);
+        forall p :: behaviorOutput(p) in aOutMS <==> behaviorOutput(p) in bOut
+    }   
+
+
+// lemma fullPatch(a:set<behavior>,b:set<behavior>)
+//     requires benignPatch(a,b);
+//     requires successfulPatch(b);
+//     requires completePatch(a,b);
+//     ensures safePatch(a,b);
+
+// Describes/Excludes 'bad' behaviors in the Unpatched Code (ie preBehaviors)
+    predicate RemovedBehaviors(b:behavior)
+    {
+
+       && ValidBehaviorNonTrivial(b)
+        && exists s:state,result:operand :: (&& s in b
+                                            && last(b) == s 
+                                            && ValidState(s)
+                                            && result.LV?
+                                            && result.l == "result"
+                                            && result.l in s.lvs
+                                            && ValidOperand(s,result)
+                                            && OperandContents(s,result).Int?
+                                            && OperandContents(s,result).val == 0)
+    }
+
+    predicate MiniSpec(b:behavior)
+    {
+        RemovedBehaviors(b)
+    }
+
+  
+
+
+    
+
+
+   
+
+   
+
+    
+
+
+}
